\section{Introduction}

\subsection{}
Setting the derivative of 
%
\begin{equation}
E(\textbf{w}) = \frac{1}{2} \sum_{n = 1}^{N} \left( y(x_n, \textbf{w}) - t_n \right) ^ 2
\end{equation}
%
as zero gives
%
\begin{equation}
\textbf{0} = \sum_{n = 1}^{N} \frac{\partial y(x_n, \textbf{w})}{\partial \textbf{w}} \left( y(x_n, \textbf{w}) - t_n \right).
\end{equation}
%
Substituting 
%
\begin{equation}
y(x_n, \textbf{w}) = \sum_{j = 0}^{M} w_j x_n^j
\end{equation}
%
gives
%
\begin{equation}
0 = \sum_{n = 1}^{N} x_n^i \left( \sum_{j = 0}^{M} w_j x_n^j - t_n \right).
\end{equation}
%
Therefore, we have 
%
\begin{equation}
\sum_{j = 0}^{M} A_{ij} w_j = T_i
\end{equation}
%
where
%
\begin{equation}
\begin{align}
A_{ij} &= \sum_{n = 1}^{N} x_n^{i + j}, \\
T_i &= \sum_{n = 1}^{N} x_n^i t_n.
\end{align}
\end{equation}


\subsection{}
Setting the derivative of 
%
\begin{equation}
\tilde{E}(\textbf{w}) = \frac{1}{2} \sum_{n = 1}^{N} \left( y(x_n, \textbf{w}) - t_n \right) ^ 2 + \frac{\lambda}{2} \lVert \textbf{w} \rVert ^ 2
\end{equation}
%
as zero gives
%
\begin{equation}
\textbf{0} = \sum_{n = 1}^{N} \frac{\partial y(x_n, \textbf{w})}{\partial \textbf{w}} \left( y(x_n, \textbf{w}) - t_n \right) + \lambda \textbf{w}.
\end{equation}
%
Substituting 
%
\begin{equation}
y(x_n, \textbf{w}) = \sum_{j = 0}^{M} w_j x_n^j
\end{equation}
%
gives
%
\begin{equation}
0 = \sum_{n = 1}^{N} x_n^i \left( \sum_{j = 0}^{M} w_j x_n^j - t_n \right) + \lambda w_i.
\end{equation}
%
Therefore, we have 
%
\begin{equation}
\sum_{j = 0}^{M} \tilde{A}_{ij} w_j = T_i
\end{equation}
%
where
%
\begin{equation}
\begin{align}
\tilde{A}_{ij} &= \sum_{n = 1}^{N} x_n^{i + j} + \lambda \delta_{ij}, \\
T_i &= \sum_{n = 1}^{N} x_n^i t_n.
\end{align}
\end{equation}
